Proofs.v
@@ -1,43 +1,68 @@
 From Licenta Require Import Semantics.
 From Licenta Require Import Syntax.
 
+Require Import String.
+Open Scope string_scope.
+
+Require Import List.
+Import ListNotations.
+
 Theorem apply_conflict_up_different: forall (u_p : unification_problem) (tp: term_pair),
   ~(check_conflict_and_deliver u_p = TError) /\ ~(u_p = Ubottom) ->
-  ~(UP u_p = UP (remove_conflict_term_pair tp u_p)).
+  maybe_unification_problem_eq (UP u_p) (UP (remove_conflict_term_pair tp u_p)) = false.
 Proof.
   intros. destruct H. induction u_p.
   - contradiction.
   - destruct ((check_conflict_and_deliver (Uset l))).
     -- contradiction.
-    -- unfold occurs_check. unfold remove_conflict_term_pair. injection. apply H0.
+    -- unfold occurs_check. unfold remove_conflict_term_pair. simpl. reflexivity.
 Qed.
 
 Theorem apply_occurs_check_up_different: forall (u_p : unification_problem) (tp: term_pair),
   ~(check_occurs_check_and_deliver u_p = TError) /\ ~(u_p = Ubottom) ->
-  ~(UP u_p = UP (occurs_check tp u_p)).
+  maybe_unification_problem_eq (UP u_p) (UP (occurs_check tp u_p)) = false.
 Proof.
   intros. destruct H. induction u_p.
   - contradiction.
   - destruct ((check_occurs_check_and_deliver (Uset l))).
     -- contradiction.
-    -- unfold occurs_check. unfold remove_conflict_term_pair. injection. apply H0.
+    -- unfold occurs_check. unfold remove_conflict_term_pair. simpl. reflexivity.
 Qed.
+
+Theorem deliver_tpair_means_in_list: forall (l : list term_pair) (tp: term_pair) (criterion: term -> term -> bool),
+  ~(deliver_tpair_from_list l criterion = TError) ->
+  In tp l.
+Proof.
+  intros. induction l.
+  - simpl in H. contradiction.
+  - simpl. right. apply IHl. unfold deliver_tpair_from_list. destruct term_pair_correct_for_rule.
+Admitted.
+
+Theorem delete_shortens_list: forall (l : list term_pair) (tp: term_pair),
+  deliver_tpair_from_list l term_eq = TP tp ->
+  length l = S (length (remove_decomposition_term_pair tp l)).
+Proof.
+  intros. unfold remove_decomposition_term_pair. Admitted.
+
+Theorem delete_term_list_inequality: forall (l : list term_pair) (tp: term_pair),
+  deliver_tpair_from_list l term_eq = TP tp ->
+  term_pair_list_eq l (remove_decomposition_term_pair tp l) = false.
+Proof.
+  intros. induction l.
+  - simpl in H. discriminate.
+  - simpl. induction (term_pair_eq tp a).
+    -- induction l.
+      --- reflexivity.
+      --- simpl. Search andb. apply Bool.andb_false_intro2. simpl. Admitted.
 
 Theorem apply_delete_up_different: forall (u_p : unification_problem) (tp: term_pair),
   ~(check_delete_and_deliver u_p = TError) /\ ~(u_p = Ubottom) 
   /\ (check_delete_and_deliver u_p = TP tp) ->
-  ~(UP u_p = UP (solver_delete tp u_p)).
+  maybe_unification_problem_eq (UP u_p) (UP (solver_delete tp u_p)) = false.
 Proof.
   intros. destruct H. destruct H0. induction u_p.
   - contradiction.
-  - destruct ((check_delete_and_deliver (Uset l))).
-    -- contradiction.
-    -- unfold solver_delete. unfold remove_first_appearance_term_unification_problem.
-       destruct (remove_first_appearance_term_pair_list) as [|l0] eqn: H_first_app.
-      --- injection. destruct l.
-        ----
-
-Qed.
+  - simpl in H1. simpl in H1. simpl. Admitted.
 
 Theorem neq_mup_implies_neq_up: forall (u_p u_p' : unification_problem),
   (UP u_p <> UP u_p')->
@@ -46,10 +71,10 @@ Proof.
   intros. unfold not. intros. unfold not in H. apply H. rewrite H0. reflexivity.
 Qed.
 
-Theorem progress'' : forall (m_u_p: maybe_unification_problem),
+Theorem progress : forall (m_u_p: maybe_unification_problem),
   ~(m_u_p = UError) /\
   ~(m_u_p = UP Ubottom) /\ ~(unification_problem_in_solved_form (mup_to_up m_u_p) = true) ->
-  (exists (m_u_p' : maybe_unification_problem), (maybe_apply_one_step m_u_p = m_u_p') /\ ~(m_u_p = m_u_p')).
+  (exists (m_u_p' : maybe_unification_problem), (maybe_apply_one_step m_u_p = m_u_p') /\ (maybe_unification_problem_eq m_u_p m_u_p' = false)).
 Proof.
   intros. destruct H. destruct H0. exists (maybe_apply_one_step m_u_p). split.
   - reflexivity.
@@ -60,12 +85,16 @@ Proof.
       --- simpl in H1. destruct (unification_problem_in_solved_form (Uset l)).
         ---- contradiction.
         ---- destruct (check_conflict_and_deliver (Uset l)) as [ | mtp] eqn: tp_eq_conflict.
-          2 : { apply (apply_conflict_up_different (Uset l)). split.
+          2 : { apply (apply_conflict_up_different (Uset l) mtp). split.
             - rewrite tp_eq_conflict. unfold not. intros. discriminate.
             - apply neq_mup_implies_neq_up. apply H0. }
           ----- destruct (check_occurs_check_and_deliver (Uset l)) as [ | mtp] eqn: tp_eq_occurs_check.
-            2 : { apply (apply_occurs_check_up_different (Uset l)). split.
+            2 : { apply (apply_occurs_check_up_different (Uset l) mtp). split.
               - rewrite tp_eq_occurs_check. unfold not. intros. discriminate.
               - apply neq_mup_implies_neq_up. apply H0. }
             ------ destruct (check_delete_and_deliver (Uset l)) as [ | mtp] eqn: tp_eq_delete.
-              2 : { 
+              2 : { apply (apply_delete_up_different (Uset l) mtp). split.
+                - rewrite tp_eq_delete. unfold not. intros. discriminate.
+                - split.
+                  -- apply neq_mup_implies_neq_up. apply H0.
+                  -- apply tp_eq_delete. Admitted.
